core/theories/Tactics.v
@@ -92,16 +92,29 @@ Ltac prove_program :=
   lazymatch goal with
   | [ |- Request ?op ?f |> ?c[?w] ]
     => let Hpre := fresh "Hpre" in
-       cut (precondition c op w); [ intro Hpre;
-                                    constructor; [apply Hpre |];
-                                    let sig := fresh "sig" in
-                                    let Hsig := fresh "Hsig" in
-                                    let res := fresh "res" in
-                                    let Hpost := fresh "Hpost" in
-                                    intros res Hpost;
-                                    prove_program
-                                  |]
-  | [ |- program_pure ?op |> ?c[?w] ] => constructor
-  | [ |- ?p |> ?c [?w] ] => repeat (cbn; destruct_if_when); prove_program
-  | [ |- ?x] => idtac x
+       assert (Hpre: precondition c op w); [| constructor; [apply Hpre |];
+                                              let sig := fresh "sig" in
+                                              let Hsig := fresh "Hsig" in
+                                              let res := fresh "res" in
+                                              let Hpost := fresh "Hpost" in
+                                              intros res Hpost;
+                                              prove_program
+                                           ]
+  | [ |- program_pure ?op |> ?c[?w] ]
+    => constructor
+  | [ |- ?p |> ?c [?w] ]
+    => repeat (cbn; destruct_if_when);
+       lazymatch goal with
+       | [ |- context[program_bind (program_bind ?p ?f) ?g] ]
+         => rewrite (program_eq_bind_assoc p f g); prove_program
+       | [ |- program_bind ?p ?f |> ?c [?w] ]
+         => let x := fresh "x" in
+            let w := fresh "w" in
+            let Hrun := fresh "Hrun" in
+            apply correct_program_compliant_run; [| intros x w Hrun; prove_program]
+       | [ |- _ ]
+         => prove_program
+       end
+  | [ |- _ ]
+    => auto
   end.
